Core.v
@@ -8,20 +8,6 @@ From Elo Require Import Map.
 Definition id := string.
 Definition num := nat.
 
-(* Notations *)
-
-Reserved Notation "'[' x ':=' tx ']' t"
-  (at level 20, x constr).
-Reserved Notation "t '--[' eff ']-->' t'"
-  (at level 40).
-Reserved Notation "m / t '==[' eff ']==>' m' / t'"
-  (at level 40, t at next level, eff at next level, m' at next level).
-Reserved Notation "m / ths '~~[' tid , eff ']~~>' m' / ths'"
-  (at level 40, ths at next level, tid at next level, eff at next level,
-                m' at next level).
-Reserved Notation "Gamma '|--' t 'is' T"
-  (at level 40).
-
 (* Types *)
 
 Inductive typ : Set :=
@@ -32,23 +18,9 @@ Inductive typ : Set :=
   | TY_Fun : typ -> typ -> typ
   .
 
-Declare Custom Entry elo_typ.
-Notation "<{{ T }}>" := T (T custom elo_typ at level 99).
-Notation "( x )"     := x (in custom elo_typ, x at level 99).
-Notation "x"         := x (in custom elo_typ at level 0, x constr at level 0).
-
-Notation "'Unit'"   := (TY_Unit)      (in custom elo_typ at level 0).
-Notation "'Num'"    := (TY_Num)       (in custom elo_typ at level 0).
-Notation "'&m' T"   := (TY_RefM T)    (in custom elo_typ at level 5).
-Notation "'&i' T"   := (TY_RefI T)    (in custom elo_typ at level 5).
-Notation "T1 -> T2" := (TY_Fun T1 T2) (in custom elo_typ at level 50,
-                                                right associativity).
-
 Theorem typ_eq_dec : forall (t1 t2 : typ),
   {t1 = t2} + {t1 <> t2}.
-Proof.
-  intros. decide equality; eauto.
-Qed.
+Proof. intros. decide equality; eauto. Qed.
 
 (* Terms *)
 
@@ -73,48 +45,61 @@ Proof.
   eauto using PeanoNat.Nat.eq_dec, string_dec, typ_eq_dec.
 Qed.
 
-(* Syntax *)
+(* Notations *)
 
-(* Declare Custom Entry stlc_ty. *)
+Declare Custom Entry elo_typ.
+Notation "<{{ T }}>" := T (T custom elo_typ at level 99).
+Notation "( x )"     := x (in custom elo_typ, x at level 99).
+Notation "x"         := x (in custom elo_typ at level 0, x constr at level 0).
+
+Notation "'Unit'"     := (TY_Unit)      (in custom elo_typ at level 0).
+Notation "'Num'"      := (TY_Num)       (in custom elo_typ at level 0).
+Notation "'&' T"      := (TY_RefM T)    (in custom elo_typ at level 5).
+Notation "'i&' T"     := (TY_RefI T)    (in custom elo_typ at level 5).
+Notation "T1 '-->' T2" := (TY_Fun T1 T2) (in custom elo_typ at level 50,
+                                                  right associativity).
 
 Declare Custom Entry elo.
 Notation "<{ t }>" := t (t custom elo at level 99).
-Notation "( x )"   := x (in custom elo, x at level 99).
 Notation "x"       := x (in custom elo at level 0, x constr at level 0).
 
-Notation "'unit'"                 := (TM_Unit)       (in custom elo at level 0).
-Notation "'N' n"                  := (TM_Num n)      (in custom elo at level 0,
-                                                                  n at level 0).
-Notation "'&' ad ':' T"           := (TM_Ref T ad)   (in custom elo at level 0,
-                                                   T custom elo_typ at level 0,
-                                                                 ad at level 0).
-Notation "'new' T t"              := (TM_New T t)    (in custom elo at level 0,
-                                                   T custom elo_typ at level 0,
-                                                       t custom elo at level 0).
-Notation "'*' t"                  := (TM_Load t)     (in custom elo at level 0,
-                                                       t custom elo at level 0).
-Notation "t1 '=' t2"              := (TM_Asg t1 t2)  (in custom elo at level 1,
-                                                            left associativity).
-Notation "'ID' x"                 := (TM_Id x)       (in custom elo at level 0,
-                                                                  x at level 0).
-Notation "'fun' x ':' Tx '->' t"  := (TM_Fun x Tx t) (in custom elo at level 0,
-                                                                  x at level 0,
-                                                  Tx custom elo_typ at level 0,
-                                                       t custom elo at level 0).
-Notation "t1 t2"                  := (TM_Call t1 t2) (in custom elo at level 1,
-                                                            left associativity).
-Notation "t1 ';' t2"              := (TM_Seq t1 t2)  (in custom elo at level 1,
-                                                            left associativity).
-Notation "'spawn' t"              := (TM_Spawn t)    (in custom elo at level 0,
-                                                                  t at level 0).
+Notation "'unit'"            := (TM_Unit)       (in custom elo at level 0).
+Notation "'N' n"             := (TM_Num n)      (in custom elo at level 0).
+Notation "'&' ad '::' T"     := (TM_Ref T ad)    (in custom elo at level 0,
+                                              T custom elo_typ at level 0).
+Notation "'new' T t"         := (TM_New T t)     (in custom elo at level 0,
+                                              T custom elo_typ at level 0).
+Notation "'*' t"             := (TM_Load t)     (in custom elo at level 0).
+Notation "t1 '=' t2"         := (TM_Asg t1 t2)  (in custom elo at level 70,
+                                                         no associativity).
+Notation "'ID' x"            := (TM_Id x)       (in custom elo at level 0).
+Notation "'fn' x Tx '-->' t" := (TM_Fun x Tx t)  (in custom elo at level 0,
+                                                       x constr at level 0,
+                                             Tx custom elo_typ at level 0).
+Notation "'call' t1 t2"      := (TM_Call t1 t2) (in custom elo at level 0).
+Notation "t1 ';' t2"         := (TM_Seq t1 t2)   (in custom elo at level 2,
+                                                      right associativity).
+Notation "'spawn' t"         := (TM_Spawn t)    (in custom elo at level 0).
+
+Reserved Notation "'[' x ':=' tx ']' t"
+  (at level 20, x constr).
+Reserved Notation "t '--[' eff ']-->' t'"
+  (at level 40, eff at next level, t' custom elo).
+Reserved Notation "m / t '==[' eff ']==>' m' / t'"
+  (at level 40, t at next level, eff at next level, m' at next level).
+Reserved Notation "m / ths '~~[' tid , eff ']~~>' m' / ths'"
+  (at level 40, ths at next level, tid at next level, eff at next level,
+                m' at next level).
+Reserved Notation "Gamma '|--' t 'is' T"
+  (at level 40).
 
 (* Values *)
 
 Inductive value : tm -> Prop :=
   | V_Unit : value <{ unit }> 
   | V_Num : forall n, value <{ N n }>
-  | V_Ref : forall ad T, value <{ &ad: T }>
-  | V_Fun : forall x Tx t, value <{ fun x: Tx -> t }>
+  | V_Ref : forall ad T, value <{ &ad :: T }>
+  | V_Fun : forall x Tx t, value <{ fn x Tx --> t }>
   .
 
 (* Effects *)
@@ -141,22 +126,22 @@ Local Infix "=?" := string_dec (at level 70, no associativity).
 
 Fixpoint subst (x : id) (tx t : tm) : tm :=
   match t with
-  | <{ unit }>             => t
-  | <{ N _ }>              => t
-  | <{ & _ : _ }>          => t
-  | <{ new T t' }>         => TM_New T ([x := tx] t')
-  | <{ *t' }>              => TM_Load  ([x := tx] t')
-  | <{ t1 = t2 }>          => TM_Asg   ([x := tx] t1) ([x := tx] t2)
-  | <{ ID x' }>            => if x =? x' then tx else t
-  | <{ fun x': Tx -> t' }> => if x =? x'
-                                then t 
-                                else TM_Fun x' Tx ([x := tx] t')
-  | <{ t1 t2  }>           => TM_Call  ([x := tx] t1) ([x := tx] t2)
-  | <{ t1; t2 }>           => TM_Seq   ([x := tx] t1) ([x := tx] t2)
-  (* | <{ spawn t' }>         => TM_Spawn ([x := tx] t') *)
-  | <{ spawn t' }>         => t
+  | <{ unit }>            => t
+  | <{ N _ }>             => t
+  | <{ & _ :: _ }>        => t
+  | <{ new T t' }>        => TM_New T ([x := tx] t')
+  | <{ *t' }>             => TM_Load  ([x := tx] t')
+  | <{ t1 = t2 }>         => TM_Asg   ([x := tx] t1) ([x := tx] t2)
+  | <{ ID x' }>           => if x =? x' then tx else t
+  | <{ fn x' Tx --> t' }> => if x =? x'
+                              then t 
+                              else TM_Fun x' Tx ([x := tx] t')
+  | <{ call t1 t2 }>      => TM_Call ([x := tx] t1) ([x := tx] t2)
+  | <{ t1; t2 }>          => TM_Seq  ([x := tx] t1) ([x := tx] t2)
+  (* | <{ spawn t' }>        => TM_Spawn ([x := tx] t') *)
+  | <{ spawn t' }>        => t
   end
-  where "'[' id ':=' x ']' t" := (subst id x t).
+  where "'[' x ':=' tx ']' t" := (subst x tx t).
 
 (* Operational Semantics *)
 
@@ -164,52 +149,52 @@ Inductive step : tm -> effect -> tm -> Prop :=
   (* New *)
   | ST_New1 : forall T t t' eff,
     t --[eff]--> t' ->
-    <{ new T t }> --[eff]--> <{ new T t' }>
+    <{ new T t }> --[eff]--> new T t'
 
   | ST_New : forall T ad v,
     value v ->
-    <{ new T v }> --[EF_Alloc ad v]--> <{ &ad: T }>
+    <{ new T v }> --[EF_Alloc ad v]--> &ad :: T
 
   (* Load *)
   | ST_Load1 : forall t t' eff,
     t --[eff]--> t' ->
-    <{ *t }> --[eff]--> <{ *t' }>
+    <{ *t }> --[eff]--> *t'
 
-  | ST_LoadM : forall ad t T,
-    <{ * (&ad: T) }> --[EF_Read ad t]--> t
+  | ST_Load : forall ad t T,
+    <{ * &ad :: T }> --[EF_Read ad t]--> t
 
   (* Asg *)
   | ST_Asg1 : forall t1 t1' t2 eff,
     t1 --[eff]--> t1' ->
-    <{ t1 = t2 }> --[eff]--> <{ t1' = t2 }>
+    <{ t1 = t2 }> --[eff]--> t1' = t2
 
   | ST_Asg2 : forall v t t' eff,
     value v ->
     t --[eff]--> t' ->
-    <{ v = t }> --[eff]--> <{ v = t' }>
+    <{ v = t }> --[eff]--> v = t'
 
   | ST_Asg : forall ad v T,
     value v ->
-    <{ &ad: T = v }> --[EF_Write ad v]--> <{ unit }> 
+    <{ &ad :: T = v }> --[EF_Write ad v]--> unit 
 
   (* Call *)
   | ST_Call1 : forall t1 t1' t2 eff,
     t1 --[eff]--> t1' ->
-    <{ t1 t2 }> --[eff]--> <{ t1' t2 }>
+    <{ call t1 t2 }> --[eff]--> call t1' t2
 
   | ST_Call2 : forall v t t' eff,
     value v ->
     t --[eff]--> t' ->
-    <{ v t }> --[eff]--> <{ v t' }>
+    <{ call v t }> --[eff]--> call v t'
 
   | ST_Call : forall x Tx t v,
     value v ->
-    <{ (fun x: Tx -> t) v }> --[EF_None]--> [x := v] t
+    <{ call <{ fn x Tx --> t }> v }> --[EF_None]--> ([x := v] t)
 
   (* Seq *)
   | ST_Seq1 : forall t1 t1' t2 eff,
     t1 --[eff]--> t1' ->
-    <{ t1; t2 }> --[eff]--> <{ t1'; t2 }>
+    <{ t1; t2 }> --[eff]--> t1'; t2
 
   | ST_Seq : forall v t,
     value v ->
@@ -217,7 +202,7 @@ Inductive step : tm -> effect -> tm -> Prop :=
 
   (* Spawn *)
   | ST_Spawn : forall t,
-    <{ spawn t }> --[EF_Spawn t]--> <{ unit }>
+    <{ spawn t }> --[EF_Spawn t]--> unit
 
   where "t '--[' eff ']-->' t'" := (step t eff t').
 
@@ -235,7 +220,7 @@ Ltac inversion_step :=
 (* Memory Step *)
 
 Definition mem := list tm.
-Definition getTM := get TM_Unit.
+Notation " l '[' i ']' " := (get TM_Unit l i) (at level 9).
 
 Inductive mstep : mem -> tm -> effect -> mem -> tm -> Prop :=
   | MST_None : forall m t t',
@@ -245,17 +230,17 @@ Inductive mstep : mem -> tm -> effect -> mem -> tm -> Prop :=
   | MST_Alloc : forall m t t' ad v,
     ad = length m ->
     t --[EF_Alloc ad v]--> t' ->
-    m / t ==[EF_Alloc ad v]==> (add m v) / t'
+    m / t ==[EF_Alloc ad v]==> (m +++ v) / t'
 
   | MST_Read : forall m t t' ad,
     ad < length m ->
-    t --[EF_Read ad (getTM m ad)]--> t' ->
-    m / t ==[EF_Read ad (getTM m ad)]==> m / t'
+    t --[EF_Read ad m[ad]]--> t' ->
+    m / t ==[EF_Read ad m[ad]]==> m / t'
 
   | MST_Write : forall m t t' ad v,
     ad < length m ->
     t --[EF_Write ad v]--> t' ->
-    m / t ==[EF_Write ad v]==> (set m ad v) / t'
+    m / t ==[EF_Write ad v]==> m[ad <- v] / t'
 
   where "m / t '==[' eff ']==>' m' / t'" := (mstep m t eff m' t').
 
@@ -276,13 +261,13 @@ Definition threads := list tm.
 Inductive cstep : mem -> threads -> nat -> effect -> mem -> threads -> Prop :=
   | CST_Mem : forall m m' t' ths tid eff,
       tid < length ths ->
-      m / (getTM ths tid) ==[eff]==> m' / t' ->
-      m / ths ~~[tid, eff]~~> m' / (set ths tid t')
+      m / ths[tid] ==[eff]==> m' / t' ->
+      m / ths ~~[tid, eff]~~> m' / ths[tid <- t']
 
   | CST_Spawn : forall m t' ths tid block,
       tid < length ths ->
-      (getTM ths tid) --[EF_Spawn block]--> t' ->
-      m / ths ~~[tid, EF_Spawn block]~~> m / (add (set ths tid t') block)
+      ths[tid] --[EF_Spawn block]--> t' ->
+      m / ths ~~[tid, EF_Spawn block]~~> m / (ths[tid <- t'] +++ block)
 
   where "m / ths '~~[' tid ,  eff ']~~>' m' / ths'" :=
     (cstep m ths tid eff m' ths').
@@ -313,37 +298,37 @@ Inductive well_typed_term : ctx -> tm -> typ -> Prop :=
     Gamma |-- <{ N n }> is <{{ Num }}>
 
   | T_Ref : forall Gamma ad T,
-    Gamma |-- <{ &ad: T }> is T
+    Gamma |-- <{ &ad :: T }> is T
 
   | T_NewM : forall Gamma t T,
     Gamma |-- t is T ->
-    Gamma |-- <{ new (&m T) t }> is <{{ &m T }}>
+    Gamma |-- <{ new &T t }> is <{{ &T }}>
 
   | T_NewI : forall Gamma t T,
     Gamma |-- t is T ->
-    Gamma |-- <{ new (&i T) t }> is <{{ &i T }}>
+    Gamma |-- <{ new i&T t }> is <{{ i&T }}>
 
   | T_LoadM : forall Gamma t T,
-    Gamma |-- t is <{{ &m T }}> ->
+    Gamma |-- t is <{{ &T }}> ->
     Gamma |-- <{ *t }> is T
 
   | T_LoadI : forall Gamma t T,
-    Gamma |-- t is <{{ &i T }}> ->
+    Gamma |-- t is <{{ i&T }}> ->
     Gamma |-- <{ *t }> is T
 
   | T_Asg : forall Gamma t1 t2 T,
-    Gamma |-- t1 is <{{ &m T }}> ->
+    Gamma |-- t1 is <{{ &T }}> ->
     Gamma |-- t2 is T ->
     Gamma |-- <{ t1 = t2 }> is <{{ Unit }}>
 
   | T_Fun : forall Gamma x t T Tx,
     Gamma[x <== Tx] |-- t is T ->
-    Gamma |-- <{ fun x: Tx -> t }> is <{{ Tx -> T }}>
+    Gamma |-- <{ fn x Tx --> t }> is <{{ Tx --> T }}>
 
   | T_Call : forall Gamma t1 t2 T Tx,
-    Gamma |-- t1 is <{{ Tx -> T }}> ->
+    Gamma |-- t1 is <{{ Tx --> T }}> ->
     Gamma |-- t2 is Tx ->
-    Gamma |-- <{ t1 t2 }> is T
+    Gamma |-- <{ call t1 t2 }> is T
 
   | T_Seq : forall Gamma t1 t2 T1 T2,
     Gamma |-- t1 is T1 ->
